A complete overhaul of the restricted quantifier library. Now all the tools regard   !x :: P. M x as a way of expressing   !x. x IN P ==> M x instead of   !x. P x ==> M x

src/res_quan/src/res_quanLib.sml
@@ -1,14 +1,8 @@
 structure res_quanLib :> res_quanLib =
 struct
 
- open Res_quan;
- open Cond_rewrite; 
+  local open res_quanTheory in end;
 
-   type hol_type = Type.hol_type
-   type term = Term.term
-   type thm = Thm.thm
-   type tactic = Abbrev.tactic
-   type conv = Abbrev.conv
-   type thm_tactic = Abbrev.thm_tactic
+  open res_quanTools;
 
 end;
