src/res_quan/src/res_quanTools.sig
@@ -1,0 +1,85 @@
+(* =====================================================================*)
+(* FILE          : res_rules.sig                                        *)
+(* DESCRIPTION   : Signature for restricted quantification inference    *)
+(*                 rules 					        *)
+(* AUTHOR	 : P Curzon 					        *)
+(* DATE		 : May 1993						*)
+(* UPDATED       : Joe Hurd, October 2001                               *)
+(*                                                                      *)
+(* =====================================================================*)
+
+signature res_quanTools =
+sig
+  include Abbrev
+
+  (* Term constructors/destructors *)
+  val mk_res_forall          : term * term * term -> term
+  val mk_res_exists          : term * term * term -> term
+  val mk_res_exists_unique   : term * term * term -> term
+  val mk_res_select          : term * term * term -> term
+  val mk_res_abstract        : term * term * term -> term
+  val dest_res_forall        : term -> term * term * term
+  val dest_res_exists        : term -> term * term * term
+  val dest_res_exists_unique : term -> term * term * term
+  val dest_res_select        : term -> term * term * term
+  val dest_res_abstract      : term -> term * term * term
+  val is_res_forall          : term -> bool
+  val is_res_exists          : term -> bool
+  val is_res_exists_unique   : term -> bool
+  val is_res_select          : term -> bool
+  val is_res_abstract        : term -> bool
+  val list_mk_res_forall     : (term * term) list * term -> term
+  val list_mk_res_exists     : (term * term) list * term -> term
+  val strip_res_forall       : term -> (term * term) list * term
+  val strip_res_exists       : term -> (term * term) list * term
+
+  (* Conversions *)
+  val RES_FORALL_CONV        : conv
+  val RES_EXISTS_CONV        : conv
+  val RES_EXISTS_UNIQUE_CONV : conv
+  val RES_SELECT_CONV        : conv
+  val IMP_RES_FORALL_CONV    : conv
+  val RES_FORALL_AND_CONV    : conv
+  val AND_RES_FORALL_CONV    : conv
+  val RES_FORALL_SWAP_CONV   : conv
+  val RESQ_REWRITE1_CONV     : thm list -> thm -> conv
+
+  (* Derived rules *)
+  val RESQ_HALF_SPEC         : term -> rule
+  val RESQ_HALF_SPECL        : term list -> rule
+  val RESQ_SPEC              : term -> rule
+  val RESQ_SPECL             : term list -> rule
+  val RESQ_MATCH_MP          : thm -> thm -> thm
+  val RESQ_REWR_CANON        : thm -> thm
+
+  (* Tactics *)
+  val RESQ_HALF_EXISTS_THEN  : thm_tactical
+  val RESQ_CHOOSE_THEN       : thm_tactical
+  val RESQ_STRIP_THM_THEN    : thm_tactical
+  val RESQ_GEN_THEN          : thm_tactic -> tactic
+  val RESQ_STRIP_GOAL_THEN   : thm_tactic -> tactic
+  val RESQ_STRIP_ASSUME_TAC  : thm_tactic
+  val RESQ_GEN_TAC           : tactic
+  val RESQ_STRIP_TAC         : tactic
+  val RESQ_EXISTS_TAC        : term -> tactic
+  val RESQ_IMP_RES_THEN      : thm_tactic -> thm_tactic
+  val RESQ_RES_THEN          : thm_tactic -> tactic
+  val RESQ_IMP_RES_TAC       : thm_tactic
+  val RESQ_RES_TAC           : tactic
+  val RESQ_REWRITE1_TAC      : thm_tactic
+
+  (* Restricted quantifier elimination using the simplifier *)
+  val RESQ_TAC               : tactic
+
+  (* Versions of some restricted quantifier tools using term quotations *)
+  val Q_RESQ_EXISTS_TAC      : term quotation -> tactic
+  val Q_RESQ_HALF_SPEC       : term quotation -> rule
+  val Q_RESQ_HALF_SPECL      : term quotation list -> rule
+  val Q_RESQ_SPEC            : term quotation -> rule
+  val Q_RESQ_SPECL           : term quotation list -> rule
+  val Q_RESQ_HALF_ISPEC      : term quotation -> rule
+  val Q_RESQ_HALF_ISPECL     : term quotation list -> rule
+  val Q_RESQ_ISPEC           : term quotation -> rule
+  val Q_RESQ_ISPECL          : term quotation list -> rule
+
+end;
