src/res_quan/src/res_quanTools.sml
@@ -1,0 +1,651 @@
+(* =====================================================================*)
+(* FILE: res_rules.ml	    DATE: 1 Aug 92	BY: Wai Wong		*)
+(* TRANSLATED	    	    DATE: 28 May 93	BY: Paul Curzon		*)
+(* UPDATED                  DATE: 30 Oct 01     BY: Joe Hurd            *)
+(* This file contains rules, conversions and tactics supporting		*)
+(* restricted quantifiers.   	    					*)
+(* =====================================================================*)
+
+(*
+*)
+structure res_quanTools :> res_quanTools =
+struct
+
+open HolKernel Drule Conv Tactic Tactical Thm_cont Rewrite boolSyntax
+  res_quanTheory boolTheory simpLib Cond_rewrite;
+
+infix ## THEN THENL THENC THENR ORELSER THEN_TCL ORELSE_TCL ++ ||;
+infixr -->;
+
+val bool_ss = boolSimps.bool_ss;
+val op++ = op THEN;
+val op|| = op ORELSE;
+fun f THENR g = g o f;
+fun f ORELSER g = fn x => f x handle HOL_ERR _ => g x;
+
+fun ERR function message =
+  HOL_ERR {origin_structure = "res_quanTools", origin_function = function,
+           message = message};
+
+(* ===================================================================== *)
+(* Syntactic operations on restricted quantifications.                   *)
+(* These ought to be generalised to all kinds of restrictions,           *)
+(* but one thing at a time.                                              *)
+(* --------------------------------------------------------------------- *)
+
+val (mk_res_forall, mk_res_exists, mk_res_exists_unique,
+     mk_res_select, mk_res_abstract) =
+ let fun mk_res_quan cons s (x,t1,t2) =
+      let val xty = type_of x
+          val t2_ty = type_of t2
+          val ty = (xty --> bool) --> (xty --> t2_ty)
+                    -->
+                   (if cons="RES_ABSTRACT" then (xty --> t2_ty) else
+                    if cons="RES_SELECT"   then xty else Type.bool)
+        in
+          mk_comb(mk_comb(mk_thy_const{Name=cons,Thy="bool",Ty=ty},t1),
+                  mk_abs(x,t2))
+        end
+        handle _ => raise ERR "mk_res_quan" s
+    in
+    (mk_res_quan "RES_FORALL"         "mk_res_forall",
+     mk_res_quan "RES_EXISTS"         "mk_res_exists",
+     mk_res_quan "RES_EXISTS_UNIQUE"  "mk_res_exists_unique",
+     mk_res_quan "RES_SELECT"         "mk_res_select",
+     mk_res_quan "RES_ABSTRACT"       "mk_res_abstract")
+    end;
+
+
+fun list_mk_res_forall (ress,body) =
+   (itlist (fn (v,p) => fn  b => mk_res_forall(v,p,b)) ress body)
+           handle _ => raise ERR "list_mk_res_forall" "";
+
+fun list_mk_res_exists (ress,body) =
+   (itlist (fn (v,p) => fn  b => mk_res_exists(v,p,b)) ress body)
+           handle _ => raise ERR "list_mk_res_exists" "";
+
+val (dest_res_forall, dest_res_exists, dest_res_exists_unique,
+     dest_res_select, dest_res_abstract) =
+    let fun dest_res_quan cons s =
+         let val check = assert (fn c => 
+                          let val {Name,Thy,...} = dest_thy_const c
+                          in Name=cons andalso Thy="bool"
+                          end)
+         in
+           fn tm => (let val (op1, rand1) = dest_comb tm
+                     val (op2, c1) = dest_comb op1
+                     val _ = check op2
+                     val (c2,c3) = dest_abs rand1
+                     in
+                       (c2,c1,c3)
+                     end)
+        end
+           handle _ => raise ERR "dest_res_quan" s
+    in
+    (dest_res_quan "RES_FORALL"         "dest_res_forall",
+     dest_res_quan "RES_EXISTS"         "dest_res_exists",
+     dest_res_quan "RES_EXISTS_UNIQUE"  "dest_res_exists_unique",
+     dest_res_quan "RES_SELECT"         "dest_res_select",
+     dest_res_quan "RES_ABSTRACT"       "dest_res_abstract")
+    end ;
+
+fun strip_res_forall fm =
+  let val (bv,pred,body) = dest_res_forall fm
+      val (prs, core) = strip_res_forall body
+  in ((bv, pred)::prs, core)
+  end
+  handle _ => ([],fm);
+
+fun strip_res_exists fm =
+  let val (bv,pred,body) = dest_res_exists fm
+      val (prs, core) = strip_res_exists body
+  in ((bv, pred)::prs, core)
+  end
+  handle _ => ([],fm);
+
+
+val is_res_forall        = can dest_res_forall;
+val is_res_exists        = can dest_res_exists;
+val is_res_exists_unique = can dest_res_exists_unique;
+val is_res_select        = can dest_res_select;
+val is_res_abstract      = can dest_res_abstract;
+
+(* ===================================================================== *)
+(* Conversions		    	    					 *)
+(* --------------------------------------------------------------------- *)
+
+local
+  fun RES_QUAN_CONV c tm =
+    let
+      val b = snd (dest_comb tm)
+    in
+      (if is_abs b then
+         let
+           val v = fst (dest_abs b)
+         in
+           c
+           THENC RAND_CONV (ABS_CONV (RAND_CONV BETA_CONV))
+           THENC RAND_CONV (ALPHA_CONV v)
+         end
+       else c) tm
+    end
+in
+  val RES_FORALL_CONV        = RES_QUAN_CONV (REWR_CONV RES_FORALL)
+  val RES_EXISTS_CONV        = RES_QUAN_CONV (REWR_CONV RES_EXISTS)
+  val RES_EXISTS_UNIQUE_CONV = RES_QUAN_CONV (REWR_CONV RES_EXISTS_UNIQUE)
+  val RES_SELECT_CONV        = RES_QUAN_CONV (REWR_CONV RES_SELECT)
+end;
+
+(* ---------------------------------------------------------------------     *)
+(* If conversion c maps term (--`\i.t1`--) to theorem |- (\i.t1) = (\i'.t1'),*)
+(* then RF_BODY_CONV c (--`!i :: P. t1`--) returns the theorem               *)
+(*     |- (!i :: P. t1) = (!i' :: P. t1')                                    *)
+(*                                                                           *)
+(* If conversion c maps term (--`t1`--) to the theorem |- t1 = t1',          *)
+(* then RF_CONV c (--`!i :: P. t1`--) returns the theorem                    *)
+(*     |- (!i :: P. t1) = (!i :: P. t1')                                     *)
+(* ---------------------------------------------------------------------     *)
+
+fun BOTH_CONV c = (LAND_CONV c THENC RAND_CONV c);
+fun LEFT_THENC_RIGHT c1 c2 = (LAND_CONV c1 THENC RAND_CONV c2);
+
+val RF_BODY_CONV = RAND_CONV;
+val RF_PRED_CONV = (RATOR_CONV o RAND_CONV);
+val RF_CONV = (RAND_CONV o ABS_CONV);
+fun PRED_THENC_BODY c1 c2 =
+   (((RATOR_CONV o RAND_CONV) c1) THENC ((RAND_CONV o ABS_CONV) c2));
+
+(* --------------------------------------------------------------------- *)
+(* IMP_RES_FORALL_CONV (--`!x. P x ==> t[x]`--)			 *)
+(*     |- !x. P x ==> t[x] = !x :: P. t[x]    	    			 *)
+(* --------------------------------------------------------------------- *)
+
+val IMP_RES_FORALL_CONV  = (fn tm =>
+    let val dthm = res_quanTheory.RES_FORALL
+    val (var, a) = dest_forall tm
+    val (ante,t) = dest_imp a
+    val (pred,v) = dest_comb ante
+    in
+     if not(var = v)
+     then raise ERR "IMP_RES_FORALL_CONV" "term not in the correct form"
+     else
+       SYM (RIGHT_CONV_RULE ((GEN_ALPHA_CONV var) THENC
+                             (ONCE_DEPTH_CONV BETA_CONV))
+                            (ISPECL [pred,mk_abs(var,t)] dthm))
+    end
+     handle HOL_ERR _ =>
+        raise ERR "IMP_RES_FORALL_CONV" "")
+    :conv;
+
+(* --------------------------------------------------------------------- *)
+(* RES_FORALL_AND_CONV (--`!i :: P. t1 /\ t2`--)  =                     *)
+(*     |- (!i :: P. t1 /\ t2) = (!i :: P. t1) /\ (!i :: P. t2)           *)
+(* --------------------------------------------------------------------- *)
+
+val RES_FORALL_AND_CONV = (fn tm =>
+    let val rthm = res_quanTheory.RES_FORALL_CONJ_DIST
+    val (var,pred,conj) = dest_res_forall tm
+    val (left,right) = dest_conj conj
+    val left_pred = mk_abs(var,left)
+    val right_pred = mk_abs(var,right)
+    val thm = ISPECL [pred, left_pred, right_pred] rthm
+    val c = LEFT_THENC_RIGHT
+        (RF_CONV(BOTH_CONV BETA_CONV)) (BOTH_CONV(RF_CONV BETA_CONV))
+    in
+       CONV_RULE c thm
+    end
+     handle HOL_ERR _ =>
+        raise ERR "RES_FORALL_AND_CONV" "")
+    :conv;
+
+(* --------------------------------------------------------------------- *)
+(* AND_RES_FORALL_CONV (--`(!i :: P. t1) /\ (!i :: P. t2)`--) =         *)
+(*     |- (!i :: P. t1) /\ (!i :: P. t2) = (!i :: P. t1 /\ t2)           *)
+(* --------------------------------------------------------------------- *)
+
+val AND_RES_FORALL_CONV = (fn tm =>
+    let val rthm = res_quanTheory.RES_FORALL_CONJ_DIST
+    val conj1 = rand(rator tm) and conj2 = rand tm
+    val (var1,pred1,body1) = dest_res_forall conj1
+    val (var2,pred2,body2) = dest_res_forall conj2
+    val thm = SYM(
+        ISPECL[pred1, mk_abs(var1,body1), mk_abs(var2,body2)] rthm)
+    val c = LEFT_THENC_RIGHT
+        (BOTH_CONV(RF_CONV BETA_CONV)) (RF_CONV(BOTH_CONV BETA_CONV))
+    in
+      CONV_RULE c thm
+    end
+     handle HOL_ERR _ =>
+        raise ERR "AND_RES_FORALL_CONV" "")
+    :conv;
+
+(* --------------------------------------------------------------------- *)
+(* RES_FORALL_SWAP_CONV (--`!i :: P. !j :: Q. R`--) =                         *)
+(*     |- (!i :: P. !j :: Q. R) = (!j :: Q. !i :: P. R)                  *)
+(* --------------------------------------------------------------------- *)
+
+val RES_FORALL_SWAP_CONV = (fn tm =>
+    let val rthm = res_quanTheory.RES_FORALL_REORDER
+    val (i,P,body) = dest_res_forall tm
+    val (j,Q,R) = dest_res_forall body
+    val thm1 = ISPECL [P,Q,mk_abs(i, mk_abs(j, R))] rthm
+    (* Reduce the two beta-redexes on either side of the equation. *)
+    val c1 = RF_CONV(RF_CONV(RATOR_CONV BETA_CONV THENC BETA_CONV))
+    val thm2 = CONV_RULE (LAND_CONV c1 THENC RAND_CONV c1) thm1
+    (* Rename the bound variables in the quantifications. *)
+    val c2 =
+        LAND_CONV(RF_CONV(RF_BODY_CONV(ALPHA_CONV j)) THENC
+            RF_BODY_CONV(ALPHA_CONV i)) THENC
+        RAND_CONV(RF_CONV(RF_BODY_CONV(ALPHA_CONV i)) THENC
+            RF_BODY_CONV(ALPHA_CONV j))
+    in
+     if i=j orelse free_in i Q orelse free_in j P
+     then raise ERR "RES_FORALL_SWAP" ""
+     else CONV_RULE c2 thm2
+    end
+     handle HOL_ERR _ =>
+        raise ERR "RES_FORALL_SWAP" "")
+    :conv;
+
+(* --------------------------------------------------------------------- *)
+(* RESQ_REWRITE1_CONV : thm list -> thm -> conv				 *)
+(* RESQ_REWRITE1_CONV thms thm tm	    				 *)
+(* The input theorem thm should be restricted quantified equational 	 *)
+(* theorem ie. the form suitable for RESQ_REWRITE_TAC. The input term tm *)
+(* should be an instance of the left-hand side of the conclusion of thm. *)
+(* The theorem list thms should contains theorems matching the conditions*)
+(* in the input thm. They are used to discharge the conditions. The 	 *)
+(* conditions which cannot be discharged by matching theorems will be 	 *)
+(* left in the assumption.   	    					 *)
+(* --------------------------------------------------------------------- *)
+
+fun RESQ_REWRITE1_CONV thms th =
+  (fn  tm =>
+    let val th' = CONV_RULE ((TOP_DEPTH_CONV RES_FORALL_CONV)
+        THENC (TOP_DEPTH_CONV RIGHT_IMP_FORALL_CONV)) th
+    in
+      COND_REWRITE1_CONV thms th' tm
+    end):conv;
+
+(* ===================================================================== *)
+(* Derived rules    	    	    					 *)
+(* --------------------------------------------------------------------- *)
+
+(* --------------------------------------------------------------------- *)
+(* Rule to specialize a restricted universal quantification.             *)
+(*                                                                       *)
+(*    A |- !x :: P. M x                                                  *)
+(*   -------------------  RESQ_HALF_SPEC                                 *)
+(*    A |- t IN P ==> M [t/x]                                            *)
+(*                                                                       *)
+(* --------------------------------------------------------------------- *)
+
+fun RESQ_HALF_SPEC tm = CONV_RULE RES_FORALL_CONV THENR SPEC tm;
+
+(* --------------------------------------------------------------------- *)
+(* Specialize a list of universal quantifiers which may be a mixture	 *)
+(* of ordinary or restricted in any order.				 *)
+(* --------------------------------------------------------------------- *)
+
+fun GEN_RESQ_HALF_SPECL spec res_spec =
+  let
+    fun half_specl asms [] th = foldl (uncurry DISCH) th asms
+      | half_specl asms (s :: rest) th =
+      if is_res_forall (concl th) then
+        let
+          val th = res_spec s th
+          val (a, _) = dest_imp (concl th)
+        in
+          half_specl (a :: asms) rest (UNDISCH th)
+        end
+      else if is_forall (concl th) then half_specl asms rest (spec s th)
+      else raise ERR "GEN_RESQ_HALF_SPECL" "not a universal quantifier"
+  in
+    half_specl []
+  end;
+
+val RESQ_HALF_SPECL = GEN_RESQ_HALF_SPECL SPEC RESQ_HALF_SPEC;
+
+(* --------------------------------------------------------------------- *)
+(* Rule to specialize a possibly restricted universal quantification.    *)
+(*                                                                       *)
+(*    A |- !x :: P. M x       A |- !x. M x                               *)
+(*   -------------------     --------------    RESQ_SPEC ``t``           *)
+(*    A, t IN P |- M t          A |- M t                                 *)
+(*                                                                       *)
+(* --------------------------------------------------------------------- *)
+
+fun RESQ_SPEC tm = (RESQ_HALF_SPEC tm THENR UNDISCH) ORELSER SPEC tm;
+
+(* ---------------------------------------------------------------------*)
+(* RESQ_SPECL : term list -> thm -> thm					*)
+(* An analogy to SPECL as RESQ_SEPC to SPEC.				*)
+(* Instatiate a list of possibly restricted universal quantifiers.	*)
+(* ---------------------------------------------------------------------*)
+
+val RESQ_SPECL = C (foldl (uncurry RESQ_SPEC));
+
+(* --------------------------------------------------------------------- *)
+(* RESQ_MATCH_MP : thm -> thm -> thm  					 *)
+(* RESQ_MATCH_MP (|- !x :: P. Q x) (|- t IN P) returns |- Q t  	    	 *)
+(* --------------------------------------------------------------------- *)
+
+fun RESQ_MATCH_MP th1 th2 = MATCH_MP (CONV_RULE RES_FORALL_CONV th1) th2;
+
+(* --------------------------------------------------------------------- *)
+(* RESQ_REWR_CANON : thm -> thm	    					 *)
+(* convert a theorem into a canonical form for COND_REWR_TAC		 *)
+(* --------------------------------------------------------------------- *)
+
+val RESQ_REWR_CANON =
+    COND_REWR_CANON o (CONV_RULE ((TOP_DEPTH_CONV RES_FORALL_CONV)));
+
+(* ===================================================================== *)
+(* Tactics   	    	    	    					*)
+(* --------------------------------------------------------------------- *)
+
+(* --------------------------------------------------------------------- *)
+(* Tactic to strip off a restricted existential quantification.          *)
+(*                                                                       *)
+(*    A ?- ?x :: P. t                                                    *)
+(*   ===================  RESQ_EXISTS_TAC (--`x'`--)                     *)
+(*    A ?-  x' IN P /\ t                                                 *)
+(*                                                                       *)
+(* --------------------------------------------------------------------- *)
+
+fun RESQ_EXISTS_TAC tm = CONV_TAC RES_EXISTS_CONV ++ EXISTS_TAC tm;
+
+(* --------------------------------------------------------------------- *)
+(* Tactic to strip off a restricted universal quantification.            *)
+(* User supplies a thm tactic for the x IN P theorem that results.       *)
+(* --------------------------------------------------------------------- *)
+
+fun RESQ_GEN_THEN ttac =
+  CONV_TAC RES_FORALL_CONV ++ GEN_TAC ++ DISCH_THEN ttac;
+
+(* --------------------------------------------------------------------- *)
+(* A restricted quantification version of STRIP_TAC.                     *)
+(* --------------------------------------------------------------------- *)
+
+fun RESQ_HALF_EXISTS_THEN (ttac : thm_tactic) =
+  ttac o CONV_RULE RES_EXISTS_CONV;
+
+val RESQ_CHOOSE_THEN =
+  RESQ_HALF_EXISTS_THEN THEN_TCL CHOOSE_THEN THEN_TCL CONJUNCTS_THEN;
+
+val RESQ_STRIP_THM_THEN = STRIP_THM_THEN ORELSE_TCL RESQ_CHOOSE_THEN;
+
+fun RESQ_STRIP_GOAL_THEN ttac = STRIP_GOAL_THEN ttac || RESQ_GEN_THEN ttac;
+
+val RESQ_STRIP_ASSUME_TAC = REPEAT_TCL RESQ_STRIP_THM_THEN CHECK_ASSUME_TAC;
+
+val RESQ_STRIP_TAC = RESQ_STRIP_GOAL_THEN RESQ_STRIP_ASSUME_TAC;
+
+(* --------------------------------------------------------------------- *)
+(* Tactic to strip off a restricted universal quantification.            *)
+(* Uses RESQ_STRIP_ASSUME_TAC to add |- x IN P to the assumptions.       *)
+(*                                                                       *)
+(*    A ?- !x :: P. t                                                    *)
+(*   ===================  RESQ_GEN_TAC                                   *)
+(*    A, x IN P ?- t                                                     *)
+(*                                                                       *)
+(* --------------------------------------------------------------------- *)
+
+val RESQ_GEN_TAC = RESQ_GEN_THEN RESQ_STRIP_ASSUME_TAC;
+
+(* --------------------------------------------------------------------- *)
+(* RESOLUTION								*)
+(* --------------------------------------------------------------------- *)
+
+(* --------------------------------------------------------------------- *)
+(* check st l : Fail with st if l is empty, otherwise return l.		*)
+(* --------------------------------------------------------------------- *)
+
+local fun check st l = if null l then raise ERR "check" st else l
+
+(* --------------------------------------------------------------------- *)
+(* check_res th : Fail if th is not in the form:			*)
+(* !x0 ... xn. !y :: P. t   otherwise, it returns the following theorem	*)
+(* !x0 ... xn y. P ==> t.    	    					*)
+(* --------------------------------------------------------------------- *)
+
+and  check_res th =
+    if is_forall (concl th) then
+    	GEN_ALL (CONV_RULE RES_FORALL_CONV (SPEC_ALL th))
+    else CONV_RULE RES_FORALL_CONV th
+      handle _ => raise ERR "check_res" "not restricted forall";
+in
+
+(* --------------------------------------------------------------------- *)
+(* RESQ_IMP_RES_THEN  : Resolve a restricted quantified theorem against	 *)
+(* the assumptions.	    	    					 *)
+(* --------------------------------------------------------------------- *)
+
+fun RESQ_IMP_RES_THEN ttac resth =
+    let val th = check_res resth
+    in IMP_RES_THEN ttac th
+    end
+    handle HOL_ERR{message = s,...} =>
+        raise ERR "RESQ_IMP_RES_THEN" s
+
+(* --------------------------------------------------------------------- *)
+(* RESQ_RES_THEN : Resolve all restricted universally quantified 	 *)
+(* assumptions against the rest.	    			 	 *)
+(* --------------------------------------------------------------------- *)
+
+and RESQ_RES_THEN (ttac:thm_tactic) (asl,g) =
+    let val a = map ASSUME asl
+    val ths = mapfilter check_res a
+    val imps = check "RESQ_RES_THEN: no restricted quantification " ths
+    val l = itlist (fn th=>append (mapfilter (MATCH_MP th) a)) imps []
+    val res = check "RESQ_RES_THEN: no resolvents " l
+    val tacs = check "RESQ_RES_THEN: no tactics" (mapfilter ttac res)
+    in
+        EVERY tacs (asl,g)
+    end
+end;
+
+fun RESQ_IMP_RES_TAC th g =
+    RESQ_IMP_RES_THEN (REPEAT_GTCL RESQ_IMP_RES_THEN STRIP_ASSUME_TAC) th g
+    handle _ => ALL_TAC g;
+
+fun RESQ_RES_TAC g =
+    RESQ_RES_THEN (REPEAT_GTCL RESQ_IMP_RES_THEN STRIP_ASSUME_TAC) g
+    handle _ => ALL_TAC g;
+
+(* --------------------------------------------------------------------- *)
+(* RESQ_REWRITE1_TAC : thm_tactic					 *)
+(* RESQ_REWRITE1_TAC |- !x::P. u[x] = v[x]				 *)
+(* transforms the input restricted quantified theorem to implicative     *)
+(* form then do conditional rewriting.					 *)
+(* --------------------------------------------------------------------- *)
+
+fun RESQ_REWRITE1_TAC th' =
+    let val th = RESQ_REWR_CANON th'
+    in
+      COND_REWR_TAC search_top_down th
+    end;
+
+(* --------------------------------------------------------------------- *)
+(* Restricted quantifier elimination using the simplifier.               *)
+(* --------------------------------------------------------------------- *)
+
+val DISCH_CONJ_CONV = REWR_CONV AND_IMP_INTRO;
+
+val UNDISCH_CONJUNCTS_TAC =
+  POP_ASSUM MP_TAC ++ REPEAT (POP_ASSUM MP_TAC ++ CONV_TAC DISCH_CONJ_CONV);
+
+fun ASMLIST_CASES (t1:tactic) _ (g as ([], _)) = t1 g
+  | ASMLIST_CASES _ t2 (g as (x::_, _)) = t2 x g;
+
+fun POP_ASSUM_TAC tac =
+  ASMLIST_CASES tac
+  (K (UNDISCH_CONJUNCTS_TAC
+      ++ tac
+      ++ TRY (DISCH_THEN (EVERY o map ASSUME_TAC o CONJUNCTS))));
+
+val RESQ_TAC =
+  POP_ASSUM_TAC
+  (SIMP_TAC bool_ss [RES_EXISTS_UNIQUE, RES_FORALL, RES_EXISTS, RES_SELECT]);
+
+(* ===================================================================== *)
+(* Functions for making definition with restrict universal quantified	 *)
+(* variables.	    	    	    					 *)
+(* The auxiliary functions used here are taken from the system directly. *)
+(* --------------------------------------------------------------------- *)
+
+(* check that tm is a <varstruct> where:
+
+   <varstruct> ::= <var> | (<varstruct>,...,<varstruct>)
+
+  and that there are no repeated variables. Return list of variables.
+*)
+
+fun check_varstruct tm =
+  if is_var tm
+  then [tm]
+  else
+   let val (t1,t2) = pairSyntax.dest_pair tm
+               handle _ => raise ERR "check_varstruct" "bad varstruct"
+
+   val l1 = check_varstruct t1
+   val l2 = check_varstruct t2
+   in
+    if intersect l1 l2 = []
+    then l1@l2
+    else raise ERR "check_varstruct" "repeated variable in varstruct"
+   end;
+
+(* check that tm is a <lhs> where:
+
+   <lhs> ::= <var> | <lhs> <varstruct>
+
+ and that no variables are repeated. Return list of variables.
+*)
+
+fun check_lhs tm =
+ if is_var tm then [tm] else 
+ if is_const tm
+ then raise ERR "check_lhs" ("attempt to redefine the constant " ^
+                             fst (dest_const tm))
+ else if not(is_comb tm)
+ then raise ERR "check_lhs" "lhs not of form (--`x = ...`--) or (--`f x = ... `--)"
+ else
+  let val (t1,t2) = dest_comb tm
+      val l1 = check_lhs t1
+      val l2 = check_varstruct t2
+  in
+     if intersect l1 l2 = []
+     then l1@l2
+     else raise ERR "check_lhs" "var used twice"
+  end;
+
+(*  if (--`C ... = (...:ty)`--) then  (get_type (--`C ...`--) ty) gives the
+   type of C.
+*)
+
+fun get_type left rightty =
+  if is_var left then rightty
+  else get_type (rator left)  (type_of(rand left) --> rightty)
+  handle _ => raise ERR "get_type" "bad lhs";
+
+(* ---------------------------------------------------------------------*)
+(* RESQ_DEF_EXISTS_RULE `!x1::P1. ... !xn::Pn. 			        *)
+(*   C y x1 ... xn z = t[y,x1,...,xn,z]`returns a theorem which is      *)
+(* suitable to be used in new_specification				*)
+(* If there are free variables in Pi, then Skolem conversion will be 	*)
+(* done, so the constant C will become C' m where m is free in Pi.	*)
+(* ---------------------------------------------------------------------*)
+
+fun RESQ_DEF_EXISTS_RULE tm =
+    let val (gvars,tm') = strip_forall tm
+    val (ress,(lh,rh)) = ((I ## dest_eq) o strip_res_forall) tm'
+    	handle _ => raise ERR "RESQ_DEF_EXISTS_RULE" "definition not an equation"
+    val leftvars = check_lhs lh
+    val cty = get_type lh (type_of rh)
+    val rightvars = free_vars rh
+    val resvars = map fst ress
+    val finpred = mk_set (flatten (map (free_vars o snd) ress))
+    val pConst = hd leftvars
+    val cname = fst(dest_var pConst)
+    in
+    if not(Lexis.allowed_term_constant cname) then
+    	raise ERR "RESQ_DEF_EXISTS_RULE" (cname^" is not allowed as a constant name")
+    else if (mem pConst resvars) then
+    	raise ERR "RESQ_DEF_EXISTS_RULE" (cname^" is restrict bound")
+    else if not(all (fn x => mem x leftvars) resvars) then
+    	raise ERR "RESQ_DEF_EXISTS_RULE" "restrict bound var not in lhs"
+    else if not(set_eq(intersect
+    	(union finpred leftvars) rightvars)rightvars) then
+    	raise ERR "RESQ_DEF_EXISTS_RULE" "unbound var in rhs"
+    else if mem(hd leftvars)rightvars then
+    	raise ERR "RESQ_DEF_EXISTS_RULE" "recursive definitions not allowed"
+    else if not(null(subtract (type_vars_in_term rh)
+                              (type_vars_in_term pConst))) then
+    	raise ERR "RESQ_DEF_EXISTS_RULE"
+          (dest_vartype(hd(subtract (type_vars_in_term rh)
+           (type_vars_in_term pConst))) ^
+           "an unbound type variable in definition")
+    else
+      let val gl = list_mk_forall (finpred,
+                    mk_exists(pConst, list_mk_res_forall
+                      (ress, list_mk_forall 
+                              (subtract(tl leftvars) resvars, mk_eq(lh,rh)))))
+      val ex = list_mk_abs((tl leftvars), rh)
+      val defthm = prove(gl,
+    	REPEAT GEN_TAC THEN EXISTS_TAC ex THEN BETA_TAC
+    	THEN REPEAT RESQ_GEN_TAC THEN REPEAT GEN_TAC THEN REFL_TAC)
+      in
+       if is_forall(concl defthm)
+       then CONV_RULE SKOLEM_CONV defthm
+       else defthm
+      end
+    end
+     handle HOL_ERR {message = s,...} =>
+        raise ERR "RESQ_DEF_EXISTS_RULE" s;
+
+(* --------------------------------------------------------------------- *)
+(* new_gen_resq_definition flag (name, (--`!x1::P1. ... !xn::Pn. 	 *)
+(*   C y x1 ... xn z = t[y,x1,...,xn,z]`--))				 *)
+(* This makes a new constant definition via new_specification.		 *)
+(*  The definition is stored in the current theory under the give name.  *)
+(*  flag specifies the syntactic status of the new constant. It should	 *)
+(*    be either "constant", or "infix" or "binder".			 *)
+(* --------------------------------------------------------------------- *)
+
+open Parse
+
+fun new_gen_resq_definition flag (name, tm) = let
+  val def_thm = RESQ_DEF_EXISTS_RULE tm
+  val cname = (fst o dest_var o fst o dest_exists o concl) def_thm
+in
+
+  new_specification {name=name,
+                     consts= [{fixity = flag, const_name = cname}],
+                     sat_thm = def_thm}
+end;
+
+val new_resq_definition =  new_gen_resq_definition Prefix;
+
+fun new_infixl_resq_definition (name,tm,fix) =
+    new_gen_resq_definition (Infixl fix) (name,tm);
+fun new_infixr_resq_definition (name,tm,fix) =
+    new_gen_resq_definition (Infixr fix) (name,tm);
+
+val new_binder_resq_definition =  new_gen_resq_definition Binder;
+
+(* --------------------------------------------------------------------- *)
+(* Some restricted quantifier functions using term quotations            *)
+(* --------------------------------------------------------------------- *)
+
+fun Q_RESQ_EXISTS_TAC tm = CONV_TAC RES_EXISTS_CONV ++ Q.EXISTS_TAC tm;
+fun Q_RESQ_HALF_SPEC tm = CONV_RULE RES_FORALL_CONV THENR Q.SPEC tm;
+val Q_RESQ_HALF_SPECL = GEN_RESQ_HALF_SPECL Q.SPEC Q_RESQ_HALF_SPEC;
+fun Q_RESQ_SPEC tm = (Q_RESQ_HALF_SPEC tm THENR UNDISCH) ORELSER Q.SPEC tm;
+val Q_RESQ_SPECL = C (foldl (uncurry Q_RESQ_SPEC));
+fun Q_RESQ_HALF_ISPEC tm = CONV_RULE RES_FORALL_CONV THENR Q.ISPEC tm;
+val Q_RESQ_HALF_ISPECL = GEN_RESQ_HALF_SPECL Q.ISPEC Q_RESQ_HALF_ISPEC;
+fun Q_RESQ_ISPEC tm = (Q_RESQ_HALF_ISPEC tm THENR UNDISCH) ORELSER Q.ISPEC tm;
+val Q_RESQ_ISPECL = C (foldl (uncurry Q_RESQ_ISPEC));
+
+end; (* res_quanTools *)
